coq/proof/SoundForgetMemory.v
@@ -1,0 +1,110 @@
+Require Import syntax.
+Require Import alist.
+Require Import FMapWeakList.
+
+Require Import Classical.
+Require Import Coqlib.
+Require Import infrastructure.
+Require Import Metatheory.
+Import LLVMsyntax.
+Import LLVMinfra.
+Require Import opsem.
+
+Require Import sflib.
+Require Import paco.
+Import Opsem.
+
+Require Import TODO.
+Require Import Exprs.
+Require Import Hints.
+Require Import Postcond.
+Require Import Validator.
+Require Import GenericValues.
+Require InvMem.
+Require InvState.
+Require Import Inject.
+Require Import SoundBase.
+Require Import SoundForget.
+
+Set Implicit Arguments.
+
+
+Definition noalias_with_def_memory (conf:Config) (def_memory:option (GenericValue * typ)) (ptr:GenericValue) (ty:typ): Prop :=
+  forall gptr_def ty_def
+         (DEF: def_memory = Some (gptr_def, ty_def)),
+    InvState.Unary.sem_noalias conf gptr_def ptr ty_def ty.
+
+Inductive state_equiv_except_mem (conf:Config) (def_mptr:option (GenericValue * typ)) (st0 st1:State): Prop :=
+| state_equiv_except_mem_intro
+    (LOCALS: st0.(EC).(Locals) = st1.(EC).(Locals))
+    (MEM: forall ptr ty a gv
+                 (NOALIAS: noalias_with_def_memory conf def_mptr ptr ty)
+                 (LOAD: mload conf.(CurTargetData) st0.(Mem) ptr ty a = Some gv),
+        mload conf.(CurTargetData) st1.(Mem) ptr ty a = Some gv)
+.
+
+Definition unique_preserved_mem conf st inv: Prop :=
+  forall u (MEM: AtomSetImpl.mem u inv.(Invariant.unique) = true),
+    InvState.Unary.sem_unique conf st u.
+
+Definition ptr_to_genericvalue conf st invst ptr: option (GenericValue * typ) :=
+  match InvState.Unary.sem_valueT conf st invst ptr.(fst) with
+  | Some gv => Some (gv, ptr.(snd))
+  | None => None
+  end.
+
+Lemma forget_memory_unary_sound
+      conf st0 invst0 invmem0 inv0
+      def_memory st1 public
+        (STATE: InvState.Unary.sem conf st0 invst0 invmem0 inv0)
+        (MEM_EQUIV: state_equiv_except_mem conf
+                    (ptr_to_genericvalue conf st0 invst0 def_memory) st0
+                    st1)
+        (UNIQUE_PRSV: unique_preserved_mem conf st1 inv0)
+    : exists invmem1,
+      <<STATE_UNARY: InvState.Unary.sem conf st1 invst0 invmem1 (ForgetMemory.unary def_memory inv0)>> /\
+      <<MEM_UNARY: InvMem.Unary.sem conf public st1.(Mem) invmem1>> /\
+      <<MEMLE_UNARY: InvMem.Unary.le invmem0 invmem1>>.
+Proof.
+Admitted.
+
+Lemma forget_memory_sound
+      conf_src st0_src st1_src def_memory_src
+      conf_tgt st0_tgt st1_tgt def_memory_tgt
+      invst0 invmem0 inv0
+      (STATE: InvState.Rel.sem conf_src conf_tgt st0_src st0_tgt invst0 invmem0 inv0)
+      (MEM: InvMem.Rel.sem conf_src conf_tgt st0_src.(Mem) st0_tgt.(Mem) invmem0)
+      (MEM_EQUIV_SRC: state_equiv_except_mem
+                  conf_src
+                  (monad.mbind _ _ (ptr_to_genericvalue conf_src st0_src invst0.(InvState.Rel.src)) def_memory_src)
+                  st0_src st1_src)
+      (MEM_EQUIV_TGT: state_equiv_except_mem
+                  conf_tgt
+                  (monad.mbind _ _ (ptr_to_genericvalue conf_tgt st0_tgt invst0.(InvState.Rel.tgt)) def_memory_tgt)
+                  st0_tgt st1_tgt)
+      (UNIQUE_PRSV_SRC: unique_preserved_mem conf_src st1_src inv0.(Invariant.src))
+      (UNIQUE_PRSV_TGT: unique_preserved_mem conf_tgt st1_tgt inv0.(Invariant.tgt))
+  : exists invmem1,
+    <<STATE: InvState.Rel.sem conf_src conf_tgt st1_src st1_tgt invst0 invmem1
+                              (ForgetMemory.t def_memory_src def_memory_tgt inv0) >> /\
+    <<MEM: InvMem.Rel.sem conf_src conf_tgt st1_src.(Mem) st1_tgt.(Mem) invmem1>> /\
+    <<MEMLE: InvMem.Rel.le invmem0 invmem1>>.
+Proof.
+  inv STATE.
+  unfold ForgetMemory.t.
+  destruct def_memory_src as [[]|], def_memory_tgt as [[]|]; ss.
+  - exploit forget_memory_unary_sound; try exact SRC; eauto. i. des.
+    exploit forget_memory_unary_sound; try exact TGT; eauto. i. des.
+    eexists (InvMem.Rel.mk _ _ _). splits; swap 2 3.
+    + econs; ss; eauto. i.
+      hexploit MAYDIFF; eauto. i.
+      admit. (* easy; use H *)
+    + econs; ss; eauto.
+    + econs; ss; eauto.
+      inv MEM.
+      admit. (* hard; use INJECT *)
+      (* state_equiv_except_mem st0 st1 (Some (ptr, ty, a, v)) -> *)
+  - admit.
+  - admit.
+  - admit.
+Admitted.
