coq/proof/SoundPostcondCmd.v
@@ -24,7 +24,8 @@ Require InvMem.
 Require InvState.
 Require Import Inject.
 Require Import SoundBase.
-Require Import SoundPostcondForget.
+Require Import SoundForget.
+Require Import SoundForgetMemory.
 Require Import SoundPostcondCmdAdd.
 
 Set Implicit Arguments.
@@ -51,6 +52,145 @@ Proof.
   inv STEP; ss. inv CMDS. ss.
 Qed.
 
+(* TODO: move this *)
+Lemma AtomSetImpl_from_list_spec1 x l
+  : AtomSetImpl.In x (AtomSetImpl_from_list l) <-> In x l.
+Proof.
+Admitted.
+
+Lemma AtomSetImpl_from_list_spec2 x l
+  : ~ AtomSetImpl.In x (AtomSetImpl_from_list l) <-> ~ In x l.
+Proof.
+Admitted.
+
+Lemma AtomSetImpl_singleton_mem_false x y
+  : AtomSetImpl.mem x (AtomSetImpl_from_list [y]) = false -> x <> y.
+Proof.
+  i.
+  apply AtomSetFacts.not_mem_iff in H.
+  apply AtomSetImpl_from_list_spec2 in H.
+  apply elim_not_In_cons in H. eauto.
+Qed.
+
+Lemma step_state_equiv_except
+      conf st0 st1 evt
+      cmd cmds
+      (NONCALL: Instruction.isCallInst cmd = false)
+      (CMDS : CurCmds st0.(EC) = cmd :: cmds)
+      (STEP: sInsn conf st0 st1 evt)
+  : state_equiv_except (AtomSetImpl_from_list (Cmd.get_def cmd))
+                       st0 (mkState st1.(EC) st1.(ECS) st0.(Mem)).
+Proof.
+  inv STEP; ss;
+    inv CMDS; econs; ss; ii;
+      hexploit AtomSetImpl_singleton_mem_false; eauto; i;
+        eauto using lookupAL_updateAddAL_neq.
+Qed.
+
+Ltac specialize_unique :=
+  match goal with
+  | [H1: AtomSetImpl.For_all (InvState.Unary.sem_unique _ _) ?inv,
+         H2: AtomSetImpl.mem ?x ?inv = true |- _] =>
+    apply AtomSetFacts.mem_iff in H2;
+    specialize (H1 _ H2)
+  end.
+
+Lemma step_unique_preserved_except
+      conf st0 st1 evt inv0
+      cmd cmds
+      (STATE: AtomSetImpl.For_all (InvState.Unary.sem_unique conf st0)
+                                  inv0.(Invariant.unique))
+      (NONCALL: Instruction.isCallInst cmd = false)
+      (CMDS : CurCmds st0.(EC) = cmd :: cmds)
+      (STEP : sInsn conf st0 st1 evt)
+  : unique_preserved_except conf inv0 (mkState st1.(EC) st1.(ECS) st0.(Mem))
+                            (AtomSetImpl_from_list (Cmd.get_def cmd))
+                            (AtomSetImpl_from_list (Cmd.get_leaked_ids cmd)).
+Proof.
+  inv STEP; ss.
+  {
+    inv CMDS.
+    ii.
+
+    apply AtomSetFacts.mem_iff in MEM.
+    specialize (STATE _ MEM).
+
+    inv STATE. ss.
+    econs; ss; eauto.
+  }
+  {
+    inv CMDS.
+    ii.
+    rewrite AtomSetFacts.union_b in NO_LEAK. ss.
+    solve_des_bool.
+    apply AtomSetImpl_singleton_mem_false in NO_LEAK.
+
+    specialize_unique.
+    inv STATE.
+
+    econs; ss.
+    - rewrite <- lookupAL_updateAddAL_neq; eauto.
+    - i.
+      destruct (id_dec id0 reg).
+      + admit.
+      + exploit LOCALS; eauto.
+        rewrite <- lookupAL_updateAddAL_neq in *; eauto.
+    - i. eauto.
+  }
+  (* TODO: result of inst not containing unique *)
+Admitted.
+
+Lemma step_equiv_except_mem
+      conf st0 st1 evt
+      cmd cmds invst
+      (NONCALL: Instruction.isCallInst cmd = false)
+      (CMDS: CurCmds st0.(EC) = cmd :: cmds)
+      (STEP: sInsn conf st0 st1 evt)
+  : state_equiv_except_mem conf
+                           (option_ptr_to_genericvalue conf (mkState st1.(EC) st1.(ECS) st0.(Mem))
+                                                       invst (Cmd.get_def_memory cmd))
+                           (mkState st1.(EC) st1.(ECS) st0.(Mem)) st1.
+Proof.
+    inv STEP; ss.
+    { econs.
+      - ss.
+      - ss.
+        i. (* TODO: malloc and mload *)
+        admit.
+    }
+    { econs.
+      - ss.
+      - ss. i.
+        unfold mload in *. des_ifs.
+        (* mload after free: use Memory.Mem.load_alloc_other. *)
+        admit.
+    }
+    { admit. (* mload after alloca *)
+    }
+    { admit. (* mload after store *) }
+    { inv CMDS. ss. }
+Admitted.
+
+Lemma step_unique_preserved_mem
+      conf st0 st1 evt
+      cmd cmds inv0
+      (STATE: AtomSetImpl.For_all (InvState.Unary.sem_unique conf (mkState st1.(EC) st1.(ECS) st0.(Mem)))
+                                  inv0.(Invariant.unique))
+      (NONCALL: Instruction.isCallInst cmd = false)
+      (CMDS: CurCmds st0.(EC) = cmd :: cmds)
+      (STEP: sInsn conf st0 st1 evt)
+      (LEAKED_NOT_UNIQUE: AtomSetImpl.disjoint inv0.(Invariant.unique) (AtomSetImpl_from_list (Cmd.get_leaked_ids cmd)))
+  : unique_preserved_mem conf st1 inv0.
+Proof.
+  inv STEP; ss;
+    try (inv CMDS; ss;
+         ii; specialize_unique; eauto).
+  { admit. (* load malloc -> undef *) }
+  { admit. (* load after free: use Memory.Mem.load_free_2 maybe *) }
+  { admit. (* load alloca *) }
+  { admit. (* load after store *) }
+Admitted.
+
 Lemma postcond_cmd_sound
       conf_src st0_src cmd_src cmds_src
       conf_tgt st0_tgt cmd_tgt cmds_tgt
@@ -73,26 +213,37 @@ Lemma postcond_cmd_sound
 Proof.
   exploit postcond_cmd_is_call; eauto. i.
   unfold postcond_cmd in *. simtac.
+  match goal with
+  | [H: Instruction.isCallInst cmd_src = false |- _] =>
+    rename H into NONCALL_SRC
+  end.
 
   destruct (s_isFinialState conf_src st0_src) eqn:FINAL.
   { unfold s_isFinialState in FINAL. simtac. }
-  exploit nerror_nfinal_nstuck; eauto. i. des.
+  exploit nerror_nfinal_nstuck; eauto. intros [st1_src]. i. des.
   replace e with evt in *; cycle 1.
   { unfold postcond_cmd_check in COND. simtac.
     exploit (@noncall_event conf_src); eauto. i.
     exploit (@noncall_event conf_tgt); eauto. i.
     subst. ss.
   }
-
-  exploit postcond_cmd_forget_sound; eauto.
-  { exploit step_state_equiv_except; eauto. }
-  { exploit step_state_equiv_except; eauto. }
-  { admit. }
-  { admit. }
-  { admit. }
-  { admit. }
+  exploit forget_sound; eauto.
+  { hexploit step_state_equiv_except; try exact CMDS_SRC; eauto. }
+  { hexploit step_state_equiv_except; try exact CMDS_TGT; eauto. }
+  { inv STATE. inv SRC. hexploit step_unique_preserved_except; try exact CMDS_SRC; eauto. }
+  { inv STATE. inv TGT. hexploit step_unique_preserved_except; try exact CMDS_TGT; eauto. }
+  intro STATE_FORGET. des.
+  exploit forget_memory_sound; try exact STATE_FORGET; eauto.
+  { hexploit step_equiv_except_mem; try exact NONCALL_SRC; eauto. }
+  { hexploit step_equiv_except_mem; try exact NONCALL_TGT; eauto. }
+  { inv STATE_FORGET.
+    hexploit step_unique_preserved_mem; try exact NONCALL_SRC; inv SRC; eauto.
+    apply forget_unique_leak_disjoint.
+  }
+  { inv STATE_FORGET.
+    hexploit step_unique_preserved_mem; try exact NONCALL_TGT; inv TGT; eauto.
+    apply forget_unique_leak_disjoint.
+  }
   i. des.
-
-  exploit postcond_cmd_add_sound; eauto. i. des.
-  esplits; eauto. etransitivity; eauto.
+  (* TODO: add lessdef_add *)
 Admitted.
